examples/nsl_pk/DY.Example.NSL.SecurityProperties.fst
@@ -62,9 +62,9 @@ val n_a_secrecy:
   (requires
     attacker_knows tr n_a /\
     trace_invariant tr /\ (
-      (exists sess_id. typed_state_was_set tr nsl_session_label alice sess_id (InitiatorSentMsg1 bob n_a)) \/
-      (exists sess_id n_b. typed_state_was_set tr nsl_session_label alice sess_id (InitiatorSentMsg3 bob n_a n_b)) \/
-      (exists sess_id n_b. typed_state_was_set tr nsl_session_label bob sess_id (ResponderReceivedMsg3 alice n_a n_b))
+      (exists sess_id. typed_state_was_set tr nsl_session_tag alice sess_id (InitiatorSentMsg1 bob n_a)) \/
+      (exists sess_id n_b. typed_state_was_set tr nsl_session_tag alice sess_id (InitiatorSentMsg3 bob n_a n_b)) \/
+      (exists sess_id n_b. typed_state_was_set tr nsl_session_tag bob sess_id (ResponderReceivedMsg3 alice n_a n_b))
     )
   )
   (ensures is_corrupt tr (principal_label alice) \/ is_corrupt tr (principal_label bob))
@@ -80,9 +80,9 @@ val n_b_secrecy:
   (requires
     attacker_knows tr n_b /\
     trace_invariant tr /\ (
-      (exists sess_id n_a. typed_state_was_set tr nsl_session_label bob sess_id (ResponderSentMsg2 alice n_a n_b)) \/
-      (exists sess_id n_a. typed_state_was_set tr nsl_session_label bob sess_id (ResponderReceivedMsg3 alice n_a n_b)) \/
-      (exists sess_id n_a. typed_state_was_set tr nsl_session_label alice sess_id (InitiatorSentMsg3 bob n_a n_b))
+      (exists sess_id n_a. typed_state_was_set tr nsl_session_tag bob sess_id (ResponderSentMsg2 alice n_a n_b)) \/
+      (exists sess_id n_a. typed_state_was_set tr nsl_session_tag bob sess_id (ResponderReceivedMsg3 alice n_a n_b)) \/
+      (exists sess_id n_a. typed_state_was_set tr nsl_session_tag alice sess_id (InitiatorSentMsg3 bob n_a n_b))
     )
   )
   (ensures is_corrupt tr (principal_label alice) \/ is_corrupt tr (principal_label bob))
